src/CancelTac.v
@@ -1,0 +1,294 @@
+Require Import List.
+Require Import Word Memory.
+Require Import Expr SepExpr SepHeap SepCancel.
+Require Import Prover.
+Require Import Tactics Reflection.
+Require ExprUnify.
+
+Set Implicit Arguments.
+Set Strict Implicit.
+
+Module CancellerTac (C : Canceller).
+  Module SH_FACTS := SepHeap.SepHeapFacts C.SH.
+  
+Section existsSubst.
+  Variable types : list type.
+  Variable funcs : functions types.
+  Variable meta_base : env types.
+  Variable var_env : env types.
+  Variable sub : C.U.Subst types.
+ 
+  Definition ExistsSubstNone (_ : tvar) (_ : expr types) := 
+    False.
+
+  Fixpoint substInEnv (from : nat) (vals : env types) (ret : env types -> Prop) : Prop :=
+    match vals with 
+      | nil => ret nil
+      | val :: vals =>
+        match C.U.Subst_lookup from sub with
+          | None => substInEnv (S from) vals (fun e => ret (val :: e))
+          | Some v => 
+            match exprD funcs meta_base var_env v (projT1 val) with
+              | None => ExistsSubstNone (projT1 val) v
+              | Some v' => projT2 val = v' /\ substInEnv (S from) vals (fun e => ret (existT _ (projT1 val) v' :: e))
+            end
+        end
+    end.
+
+  Fixpoint existsMaybe (vals : list { t : tvar & option (tvarD types t) }) (ret : env types -> Prop) : Prop :=
+    match vals with
+      | nil => ret nil
+      | existT t None :: vals => exists x : tvarD types t, existsMaybe vals (fun e => ret (existT _ t x :: e))
+      | existT t (Some v) :: vals => existsMaybe vals (fun e => ret (existT _ t v :: e))
+    end.
+
+End existsSubst.
+
+Definition existsSubst types funcs var_env sub (from : nat) (vals : list { t : tvar & option (tvarD types t) }) (ret : env types -> Prop) :=
+  existsMaybe vals (fun e => @substInEnv types funcs e var_env sub from e ret).
+
+Fixpoint consistent {ts} (vals : list { x : tvar & option (tvarD ts x) }) (e : list { x : tvar & tvarD ts x }) : Prop :=
+  match vals , e with
+    | nil , nil => True
+    | existT t None :: vals , existT t' _ :: e =>
+      t = t' /\ @consistent _ vals e
+    | existT t (Some v) :: vals , existT t' v' :: e =>
+      match equiv_dec t t' return Prop with
+        | left pf => 
+          v' = match (pf : t = t') in _ = t return tvarD ts t with
+                 | refl_equal => v
+               end /\ @consistent _ vals e
+        | right _ => False
+      end
+    | _ , _ => False
+  end.
+
+Lemma ex_iff : forall T (P P' : T -> Prop),
+  (forall x, P x <-> P' x) ->
+  ((exists x, P x) <-> (exists x, P' x)).
+Proof. split; intuition; destruct H0 as [ x ? ]; exists x; firstorder. Qed.
+
+Theorem existsMaybe_sem : forall types vals (ret : env types -> Prop),
+  existsMaybe vals ret <->
+  existsEach (map (@projT1 _ _) vals) (fun e => consistent vals e /\ ret e).
+Proof.
+  induction vals; simpl; intros.
+  { intuition. }
+  { destruct a. destruct o.
+    { rewrite IHvals. intuition. exists t. apply existsEach_sem. apply existsEach_sem in H.
+      destruct H. exists x0. simpl in *. rewrite EquivDec_refl_left. intuition.
+      destruct H. apply existsEach_sem. apply existsEach_sem in H. destruct H.
+      exists x1. simpl in *. rewrite EquivDec_refl_left in H. intuition; subst; auto. }
+    { simpl. eapply ex_iff. intros. rewrite IHvals.
+      intuition; apply existsEach_sem in H; apply existsEach_sem; destruct H; exists x1; intuition. } }
+Qed.
+
+Lemma substInEnv_sem : forall types funcs meta_env var_env sub vals from ret,
+  @substInEnv types funcs meta_env var_env sub from vals ret <-> 
+  (C.U.Subst_equations_to funcs meta_env var_env sub from vals /\ ret vals).
+Proof.
+  induction vals; simpl; intros.
+  { intuition. }
+  { destruct a; simpl in *.
+    consider (C.U.Subst_lookup from sub); simpl; intros.
+    consider (exprD funcs meta_env var_env e x); simpl; intros.
+    { rewrite IHvals. intuition; subst; auto. } 
+    { intuition. }
+    { rewrite IHvals. intuition. } }
+Qed.
+
+Lemma existsSubst_sem : forall ts (funcs : functions ts) vals sub vars_env from ret,
+  existsSubst funcs vars_env sub from vals ret <->
+  existsEach (map (@projT1 _ _) vals) (fun meta_env =>
+    consistent vals meta_env /\ C.U.Subst_equations_to funcs meta_env vars_env sub from meta_env /\ ret meta_env).
+Proof.
+  intros. unfold existsSubst.
+  rewrite existsMaybe_sem. rewrite existsEach_sem. rewrite existsEach_sem.
+  apply ex_iff. intros. rewrite substInEnv_sem. intuition.
+Qed.
+
+(** The actual canceller starts here **)
+Section canceller.
+  Variable types : list type.
+  Variable funcs : functions types.
+  Variable preds : C.SH.SE.predicates types.
+  Variable prover : ProverT types.
+
+  Record CancellerResult : Type :=
+  { Lhs    : C.SH.SHeap types
+  ; Rhs    : C.SH.SHeap types
+  ; Subst  : C.U.Subst types
+  }.
+  
+  Let bound := 10.
+
+  Definition canceller tpreds (facts : Facts prover)
+    (lhs rhs : C.SH.SHeap types) (sub : C.U.Subst types) : CancellerResult * bool :=
+    match C.sepCancel prover bound tpreds facts lhs rhs sub with
+      | Some (l,r,s) =>
+        ({| Lhs := l ; Rhs := r ; Subst := s |}, true)
+      | None => 
+        ({| Lhs := lhs ; Rhs := rhs ; Subst := sub |}, false)
+    end.
+
+  Lemma WellTyped_env_app : forall ts a b c d,
+    WellTyped_env a c ->
+    WellTyped_env b d ->
+    WellTyped_env (types := ts) (a ++ b) (c ++ d).
+  Proof. clear.
+    intros. unfold WellTyped_env in *. unfold typeof_env in *. subst. 
+    rewrite map_app. reflexivity.
+  Qed.
+  Ltac t_list_length := repeat (rewrite typeof_env_length || rewrite rev_length || rewrite map_length || rewrite app_length).
+  Hint Extern 1 (_ = _) => t_list_length; auto : list_length.
+
+  Ltac env_resolution :=
+    repeat (rewrite typeof_env_app || unfold typeof_env || rewrite map_app || rewrite map_rev || (f_equal; []) || assumption).
+
+  Lemma consistent_app : forall ts a b c,
+    consistent (ts := ts) (a ++ b) c ->
+    consistent a (firstn (length a) c) /\ consistent b (skipn (length a) c).
+  Proof. clear.
+    induction a; simpl; intros; auto.
+    destruct a. destruct o. destruct c; try contradiction. destruct s. destruct (equiv_dec x x0); try contradiction.
+    destruct H. eapply IHa in H0. intuition.
+    destruct c; try contradiction. destruct s. destruct H. apply IHa in H0. intuition.
+  Qed.
+  Lemma consistent_Some : forall ts a c,
+    consistent (ts := ts) (map (fun x => existT _ (projT1 x) (Some (projT2 x))) a) c ->
+    a = c.
+  Proof.
+    induction a; destruct c; simpl; intros; try contradiction; auto.
+    destruct s. destruct a; simpl in *. destruct (equiv_dec x0 x); try contradiction.
+    unfold equiv in e. intuition; subst. f_equal; eauto.
+  Qed.
+
+  Lemma ApplyCancelSep_with_eq' : forall (PC : ProverT_correct prover funcs) (meta_env var_env : env types)
+    (facts : Facts prover) (sub : C.U.Subst _),
+    Valid PC meta_env var_env facts ->
+    C.U.Subst_equations funcs meta_env var_env sub ->
+    forall (l r : C.SH.SHeap types) res prog,
+    forall (WTR : C.SH.WellTyped_sheap (typeof_funcs funcs) (C.SH.SE.typeof_preds preds) (typeof_env meta_env) (typeof_env var_env) r = true),
+    canceller (C.SH.SE.typeof_preds preds) facts l r sub = (res, prog) ->
+    match res with
+      | {| Lhs    := lhs'
+         ; Rhs    := rhs'
+         ; Subst  := subst
+         |} =>
+        existsSubst funcs var_env subst 0 
+          (map (fun x => existT (fun t => option (tvarD types t)) (projT1 x) (Some (projT2 x))) meta_env)
+          (fun meta_env : Expr.env types =>
+            C.SH.SE.ST.himp
+              (C.SH.SE.sexprD funcs preds meta_env var_env (C.SH.sheapD lhs'))
+              (C.SH.SE.sexprD funcs preds meta_env var_env (C.SH.sheapD rhs')))
+              
+    end ->
+    C.SH.SE.ST.himp (@C.SH.SE.sexprD _ funcs preds meta_env var_env (C.SH.sheapD l))
+                    (@C.SH.SE.sexprD _ funcs preds meta_env var_env (C.SH.sheapD r)).
+  Proof.
+    Opaque Env.repr.
+    intros. unfold canceller in *.
+
+    consider (C.sepCancel prover bound (C.SH.SE.typeof_preds preds) facts l r sub); intros.
+    { destruct p. destruct p. inversion H3; clear H3; subst.
+      eapply SH_FACTS.SEP_FACTS.himp_WellTyped_sexpr; intros.
+      eapply existsSubst_sem in H2.
+      rewrite map_map in *. simpl in *.
+      eapply existsEach_sem in H2. destruct H2. intuition.
+      eapply consistent_Some in H2; subst.
+
+      eapply C.sepCancel_correct in H1; try eassumption.
+      eapply C.U.Subst_equations_WellTyped; eassumption.
+      rewrite C.SH.WellTyped_sheap_WellTyped_sexpr; eassumption.
+
+      eapply C.U.Subst_equations_to_Subst_equations; eauto.
+      eapply C.sepCancel_PureFacts in H1; try eassumption; intuition.
+      eapply C.U.Subst_equations_WellTyped; eassumption.
+      rewrite C.SH.WellTyped_sheap_WellTyped_sexpr; eassumption. }
+    { inversion H3; clear H3; subst.
+      eapply SH_FACTS.himp_pull_pures; intros.
+      eapply existsSubst_sem in H2.
+      rewrite map_map in H2. simpl in H2.
+      eapply existsEach_sem in H2.
+      destruct H2. intuition.
+      eapply consistent_Some in H2; subst. eauto. }
+  Qed.
+
+(*
+  Lemma ApplyCancelSep_with_eq : 
+    forall (algos_correct : ILAlgoTypes.AllAlgos_correct funcs preds algos),
+    forall (meta_env : env (Env.repr BedrockCoreEnv.core types)) (hyps : Expr.exprs (_)),
+
+    forall (l r : SEP.sexpr types BedrockCoreEnv.pc BedrockCoreEnv.st) res,
+    canceller (typeof_env meta_env) hyps l r = Some res ->
+    Expr.AllProvable funcs meta_env nil hyps ->
+    forall (WTR : SEP.WellTyped_sexpr (typeof_funcs funcs) (SEP.typeof_preds preds) (typeof_env meta_env) nil r = true) cs,
+
+    match res with
+      | {| AllExt := new_vars
+         ; ExExt  := new_uvars
+         ; Lhs    := lhs'
+         ; Rhs    := rhs'
+         ; Subst  := subst
+         |} =>
+        Expr.forallEach new_vars (fun nvs : Expr.env types =>
+          let var_env := nvs in
+          Expr.AllProvable_impl funcs meta_env var_env
+          (existsSubst funcs var_env subst 0 
+            (map (fun x => existT (fun t => option (tvarD types t)) (projT1 x) (Some (projT2 x))) meta_env ++
+             map (fun x => existT (fun t => option (tvarD types t)) x None) new_uvars)
+            (fun meta_env : Expr.env types =>
+                (Expr.AllProvable_and funcs meta_env var_env
+                  (himp cs 
+                    (SEP.sexprD funcs preds meta_env var_env
+                      (SH.sheapD (SH.Build_SHeap _ _ (SH.impures lhs') nil (SH.other lhs'))))
+                    (SEP.sexprD funcs preds meta_env var_env
+                      (SH.sheapD (SH.Build_SHeap _ _ (SH.impures rhs') nil (SH.other rhs')))))
+                  (SH.pures rhs')) ))
+            (SH.pures lhs'))
+    end ->
+    himp cs (@SEP.sexprD _ _ _ funcs preds meta_env nil l)
+            (@SEP.sexprD _ _ _ funcs preds meta_env nil r).
+  Proof. intros. eapply ApplyCancelSep_with_eq'; eauto. Qed.
+
+  Lemma ApplyCancelSep : 
+    forall (algos_correct : ILAlgoTypes.AllAlgos_correct funcs preds algos),
+    forall (meta_env : env (Env.repr BedrockCoreEnv.core types)) (hyps : Expr.exprs (_)),
+    forall (l r : SEP.sexpr types BedrockCoreEnv.pc BedrockCoreEnv.st),
+      Expr.AllProvable funcs meta_env nil hyps ->
+    forall (WTR : SEP.WellTyped_sexpr (typeof_funcs funcs) (SEP.typeof_preds preds) (typeof_env meta_env) nil r = true) cs,
+    match canceller (typeof_env meta_env) hyps l r with
+      | Some {| AllExt := new_vars
+         ; ExExt  := new_uvars
+         ; Lhs    := lhs'
+         ; Rhs    := rhs'
+         ; Subst  := subst
+         |} =>
+        Expr.forallEach new_vars (fun nvs : Expr.env types =>
+          let var_env := nvs in
+          Expr.AllProvable_impl funcs meta_env var_env
+          (existsSubst funcs var_env subst 0 
+            (map (fun x => existT (fun t => option (tvarD types t)) (projT1 x) (Some (projT2 x))) meta_env ++
+             map (fun x => existT (fun t => option (tvarD types t)) x None) new_uvars)
+            (fun meta_env : Expr.env types =>
+                (Expr.AllProvable_and funcs meta_env var_env
+                  (himp cs 
+                    (SEP.sexprD funcs preds meta_env var_env
+                      (SH.sheapD (SH.Build_SHeap _ _ (SH.impures lhs') nil (SH.other lhs'))))
+                    (SEP.sexprD funcs preds meta_env var_env
+                      (SH.sheapD (SH.Build_SHeap _ _ (SH.impures rhs') nil (SH.other rhs')))))
+                  (SH.pures rhs')) ))
+            (SH.pures lhs'))
+      | None => 
+        himp cs (@SEP.sexprD _ _ _ funcs preds meta_env nil l)
+                (@SEP.sexprD _ _ _ funcs preds meta_env nil r)
+    end ->
+    himp cs (@SEP.sexprD _ _ _ funcs preds meta_env nil l)
+            (@SEP.sexprD _ _ _ funcs preds meta_env nil r).
+  Proof. 
+    intros. consider (canceller (typeof_env meta_env) hyps l r); intros; auto.
+    eapply ApplyCancelSep_with_eq; eauto.
+  Qed.
+*)
+
+End canceller.
